src/Inode.v
@@ -1,0 +1,110 @@
+Require Import Arith.
+Require Import Pred.
+Require Import Word.
+Require Import Prog.
+Require Import Hoare.
+Require Import SepAuto.
+Require Import BasicProg.
+Require Import Omega.
+Require Import Log.
+Require Import Array.
+Require Import List.
+Require Import Bool.
+Require Import Eqdep_dec.
+
+Set Implicit Arguments.
+
+
+(* Inode layout *)
+
+Record xparams := {
+  IXStart : addr;
+    IXLen : addr
+}.
+
+Module INODE.
+  Inductive alloc_state :=
+  | Avail
+  | InUse.
+
+  Record inode := mkinode {
+    IFree: alloc_state;
+    ILen: addr;
+    IBlocks: addr -> addr
+  }.
+
+  Definition alloc_state_to_bits a : addr :=
+    match a with
+    | Avail => $0
+    | InUse => $1
+    end.
+
+  Definition bits_to_alloc_state (a : addr) : alloc_state :=
+    if (weq a $0) then Avail else InUse.
+
+  Notation "a ^++ b" := (@Word.combine _ a _ b) (at level 55, left associativity).
+
+  Definition inodelen := (addrlen + addrlen + addrlen + addrlen).
+
+  Definition inode_pack (i : inode) : word inodelen :=
+    let (f, l, b) := i in
+    (alloc_state_to_bits f) ^++ l ^++ (b $0) ^++ (b $1).
+
+  Notation "a ^-- sz" := ((@Word.split1 sz _ a), (@Word.split2 sz _ a)) (at level 55).
+
+  Definition inode_unpack (w : word inodelen) : inode :=
+    let (f, w) := w ^-- addrlen in
+    let (l, w) := w ^-- addrlen in
+    let (b0, w) := w ^-- addrlen in
+    let (b1, w) := w ^-- addrlen in
+    mkinode (bits_to_alloc_state f) l
+            (fun x => if weq x $0 then b0 else b1).
+
+  Theorem inode_pack_unpack : forall i,
+    inode_unpack (inode_pack i) = i.
+  Proof.
+    destruct i.
+    unfold inode_unpack, inode_pack.
+    f_equal.
+    (* XXX rewrite split2_combine, split1_combine? *)
+    (* XXX not quite correct because of addrs other than $0 and $1 in IBlocks;
+     * should IBlocks be a fixed-length list instead?  or a list with an extra
+     * Prop field in inode about the length of that list?
+     *)
+  Abort.
+
+  Lemma inodelen_valulen : inodelen + (valulen - inodelen) = valulen.
+  Proof.
+    rewrite valulen_is.
+    auto.
+  Qed.
+
+  Definition inodew2valu (w : word inodelen) : valu.
+    set (zext w (valulen-inodelen)) as r.
+    rewrite inodelen_valulen in r.
+    apply r.
+  Defined.
+
+  Definition valu2inodew (v : valu) : word inodelen.
+    rewrite <- inodelen_valulen in v.
+    apply (split1 inodelen (valulen-inodelen) v).
+  Defined.
+
+  Theorem inodew2valu2inodew : forall i,
+    valu2inodew (inodew2valu i) = i.
+  Proof.
+    unfold valu2inodew, inodew2valu.
+    unfold eq_rec_r, eq_rec.
+    intros.
+    rewrite <- inodelen_valulen.
+    do 2 (rewrite <- eq_rect_eq_dec; try apply eq_nat_dec).
+    apply split1_combine.
+  Qed.
+
+  Definition rep xp (imap : addr -> inode) :=
+    array (IXStart xp)
+          (map (fun i => inode_to_valu (imap $ i)) (seq 0 (wordToNat (IXLen xp)))).
+
+
+
+End INODE.
